examples/stlc/verif.v
@@ -10,14 +10,14 @@ Open Scope coq_nat.
 (* Note : Some tactic automation would improve our proofs *)
 
 (* This could be turned into a more generic lemma, but for now it works *)
-Lemma vars_with_type_shift: 
-  forall e x tau n, 
+Lemma vars_with_type_shift:
+  forall e x tau n,
     In (Id (S x))
        (map (fun p : type * var => Id (snd p))
             (filter
                (fun p : type * nat =>
                   proj1_sig (Sumbool.bool_of_sumbool (type_eq_dec tau (fst p))))
-               (combine e (seq (S n) (length e))))) <-> 
+               (combine e (seq (S n) (length e))))) <->
     In (Id x)
        (map (fun p : type * var => Id (snd p))
             (filter
@@ -25,20 +25,20 @@ Lemma vars_with_type_shift:
                   proj1_sig (Sumbool.bool_of_sumbool (type_eq_dec tau (fst p))))
                (combine e (seq n (length e))))).
 Proof.
-  move => e. induction e; intros x tau; simpl in *; split; auto; 
+  move => e. induction e; intros x tau; simpl in *; split; auto;
   intros H; destruct (type_eq_dec tau a); subst; simpl in *;
   try (destruct H; try (inversion H; auto));
-  try right; apply IHe; auto. 
+  try right; apply IHe; auto.
 Qed.
 
-Lemma vars_with_type_le: 
-  forall e x tau n, 
+Lemma vars_with_type_le:
+  forall e x tau n,
     In (Id x)
        (map (fun p : type * var => Id (snd p))
             (filter
                (fun p : type * nat =>
                   proj1_sig (Sumbool.bool_of_sumbool (type_eq_dec tau (fst p))))
-               (combine e (seq n (length e))))) -> n <= x. 
+               (combine e (seq n (length e))))) -> n <= x.
 Proof.
   move => e. induction e; intros x tau n H; simpl in *.
   now exfalso; auto.
@@ -47,8 +47,8 @@ Proof.
   eapply IHe in H; lia.
 Qed.
 
-Lemma vars_with_type_le_length_aux: 
-  forall e x tau n, 
+Lemma vars_with_type_le_length_aux:
+  forall e x tau n,
     In (Id x)
        (map (fun p : type * var => Id (snd p))
             (filter
@@ -56,23 +56,23 @@ Lemma vars_with_type_le_length_aux:
                   proj1_sig (Sumbool.bool_of_sumbool (type_eq_dec tau (fst p))))
                (combine e (seq n (length e))))) -> x < n + (length e).
 Proof.
-  move => e. induction e; intros x tau n H; simpl in *. 
+  move => e. induction e; intros x tau n H; simpl in *.
   now exfalso; auto. unfold addn, addn_rec in *.
   destruct (type_eq_dec tau a); subst; simpl in *.
   destruct H. inversion H; subst. lia.
   apply IHe in H. lia. eapply IHe in H; lia.
 Qed.
 
-Lemma vars_with_type_le_length: 
-  forall e x tau, 
+Lemma vars_with_type_le_length:
+  forall e x tau,
     In (Id x) (vars_with_type e tau) -> x < (length e).
 Proof.
-  intros. apply vars_with_type_le_length_aux in H. 
+  intros. apply vars_with_type_le_length_aux in H.
   unfold addn, addn_rec in *. lia.
 Qed.
 
 Lemma vars_with_type_Id :
-  forall e tau t, 
+  forall e tau t,
     In t (vars_with_type e tau) -> exists x, t = Id x.
 Proof.
   intros. rewrite /vars_with_type /= in H.
@@ -81,46 +81,46 @@ Proof.
 Qed.
 
 Lemma type_var :
-  forall e x tau, In (Id x) (vars_with_type e tau) <-> typing e (Id x) tau.  
+  forall e x tau, In (Id x) (vars_with_type e tau) <-> typing e (Id x) tau.
 Proof.
-  induction e as [| tau e IHe]; move => x tau' /=. 
+  induction e as [| tau e IHe]; move => x tau' /=.
   - split; intros H;
-    solve [exfalso; auto | 
-           inversion H; subst; destruct x; simpl in *; discriminate ]. 
+    solve [exfalso; auto |
+           inversion H; subst; destruct x; simpl in *; discriminate ].
   - split; rewrite /vars_with_type /=; intros H;
     destruct (type_eq_dec tau' tau); subst.
     + destruct x; simpl in *; auto. constructor; auto.
       inversion H as [H1 | H1]; try discriminate.
-      setoid_rewrite vars_with_type_shift in H1. apply IHe in H1. 
-      inversion H1; subst. constructor; auto. 
+      setoid_rewrite vars_with_type_shift in H1. apply IHe in H1.
+      inversion H1; subst. constructor; auto.
     + destruct x; simpl in *; auto.
       constructor; auto. apply vars_with_type_le in H. lia.
-      setoid_rewrite vars_with_type_shift in H. apply IHe in H. 
-      inversion H; subst. constructor; auto. 
-    + destruct x; simpl in *; auto. 
+      setoid_rewrite vars_with_type_shift in H. apply IHe in H.
+      inversion H; subst. constructor; auto.
+    + destruct x; simpl in *; auto.
       right. rewrite vars_with_type_shift. apply IHe. inversion H. simpl in *.
       constructor; auto.
     + destruct x; simpl in *; auto. inversion H; subst.
       simpl in *.
       exfalso; auto. inversion H1; auto.
-      rewrite vars_with_type_shift. apply IHe. 
+      rewrite vars_with_type_shift. apply IHe.
       inversion H; subst. constructor; auto.
 Qed.
 
 Lemma app_free_app_no_0 :
-  forall (t : term), 
+  forall (t : term),
     app_free t <-> app_no t = 0.
 Proof.
   elim => [n | x | t1 _ t2 _ | t IHt ]; split; intros H;
   solve [ inversion H; (try apply IHt); subst; auto |
           constructor; try apply IHt; auto ].
-Qed. 
+Qed.
 
 Inductive Const_leq (s : nat) : term -> Prop :=
 | IdLe : forall x, Const_leq s (Id x)
 | ConstLe : forall n, n <= s -> Const_leq s (Const n)
 | AppLe :
-    forall t1 t2, 
+    forall t1 t2,
       Const_leq s t1 -> Const_leq s t2 ->
       Const_leq s (App t1 t2)
 | AbsLe :
@@ -128,7 +128,7 @@ Inductive Const_leq (s : nat) : term -> Prop :=
       Const_leq s t -> Const_leq s (Abs t).
 
 Fixpoint max_const (t : term) : nat :=
-  match t with 
+  match t with
     | Id _ => 0
     | Const n => n
     | App t1 t2 => max (max_const t1) (max_const t2)
@@ -136,8 +136,8 @@ Fixpoint max_const (t : term) : nat :=
   end.
 
 Lemma Const_leq_trans :
-  forall t n1 n2, 
-    n1 <= n2 -> 
+  forall t n1 n2,
+    n1 <= n2 ->
     Const_leq n1 t -> Const_leq n2 t.
 Proof.
   intros. induction t; try (constructor; simpl; lia);
@@ -155,25 +155,25 @@ Qed.
 
 Lemma gen_type_size_correctSize :
   forall (n s : nat),
-    semGenSize (gen_type_size n) s <--> [set tau | type_size tau = n]. 
+    semGenSize (gen_type_size n) s <--> [set tau | type_size tau = n].
 Proof.
   move => n s tau. elim : tau n s => [| tau1 IH1 tau2 IH2] n s.
-  { split. 
+  { split.
     - destruct n as [| n]; move => H //=.
-      move : H => /semBindSize 
+      move : H => /semBindSize
                    [m1 [/semChooseSize H1 H2]].
-      move : H2 => /semLiftGen2Size [[tau1 tau2] [[/=  H3  H4] H]]. discriminate. 
+      move : H2 => /semLiftGen2Size [[tau1 tau2] [[/=  H3  H4] H]]. discriminate.
     - move => H. destruct n as [| n]; simpl.
       apply semReturnSize. reflexivity. discriminate. }
-  { split. 
+  { split.
     - destruct n as [| n].
       + move => /semReturnSize <-. auto.
-      + move  => /semBindSize 
-                      [m1 [/semChooseSize H1 H2]]. fold gen_type_size in H2. 
+      + move  => /semBindSize
+                      [m1 [/semChooseSize H1 H2]]. fold gen_type_size in H2.
         move : H2 => /semLiftGen2Size [[tau1' tau2'] [[/=  H3  H4] Heq]].
         rewrite /set1 in Heq. inversion Heq; subst.
-        apply IH1 in H3. apply IH2 in H4.
-        have Hle1 : type_size tau1 = (n - m1)%coq_nat 
+        rewrite IH1 in H3. rewrite IH2 in H4.
+        have Hle1 : type_size tau1 = (n - m1)%coq_nat
           by apply H3; lia.
         have Hle2 : type_size tau2 = (n - (n - m1)%coq_nat)%coq_nat
           by apply H4; lia. lia.
@@ -181,19 +181,19 @@ Proof.
       apply semBindSize. exists (n - type_size tau1). split.
       apply semChooseSize; unfold leq, super, OrdNat in *.
       apply/leP. lia. apply/andP; split; apply /leP; lia.
-      apply semLiftGen2Size. exists (tau1, tau2). 
+      apply semLiftGen2Size. exists (tau1, tau2).
       split; last by reflexivity.
-      split; fold gen_type_size; [ apply IH1 | apply IH2]; 
+      split; fold gen_type_size; [ apply IH1 | apply IH2];
       simpl; simpl in H; lia. }
 Qed.
 
 Lemma gen_type_correctSize :
   forall (s : nat),
-    semGenSize gen_type s <--> [set tau | type_size tau <= s]. 
+    semGenSize gen_type s <--> [set tau | type_size tau <= s].
 Proof.
-  intros s. unfold gen_type. rewrite semBindSize => tau. 
-  split => H. 
-  - move : H => [n  [/arbNat_correctSize H1 /gen_type_size_correctSize H2]]. 
+  intros s. unfold gen_type. rewrite semBindSize => tau.
+  split => H.
+  - move : H => [n  [/arbNat_correctSize H1 /gen_type_size_correctSize H2]].
     lia.
   - exists (type_size tau). split. apply arbNat_correctSize; auto.
     apply gen_type_size_correctSize; auto.
@@ -201,15 +201,15 @@ Qed.
 
 Lemma gen_term_no_app_correctSize :
   forall (tau : type) (e : env) (s: nat),
-    semGenSize (gen_term_no_app tau e) s <--> 
+    semGenSize (gen_term_no_app tau e) s <-->
     [set t | typing e t tau /\ app_free t /\ Const_leq s t].
 Proof.
   induction tau; intros e s; simpl.
   - destruct (vars_with_type e N) as [| x e'] eqn:Hvars.
-    + rewrite semLiftGenSize. intros t'. split. 
-      * move => [n [/arbNat_correctSize Hnat <-]]. 
+    + rewrite semLiftGenSize. intros t'. split.
+      * move => [n [/arbNat_correctSize Hnat <-]].
         repeat split; constructor; auto.
-      * move =>  [H [H' H'']]; subst. 
+      * move =>  [H [H' H'']]; subst.
         inversion H; subst; (try now inversion H'); inversion H''; subst.
         apply type_var in H. rewrite Hvars in H. inversion H.
         exists n. split; try reflexivity. now apply arbNat_correctSize.
@@ -217,7 +217,7 @@ Proof.
       * move => [gen [[H1 | [ H1 | // ]] H2]]; subst.
         move /semLiftGenSize : H2 => [n [/arbNat_correctSize Hnat <-]].
         repeat split; constructor; auto.
-        apply semElementsSize in H2. 
+        setrw_hyp (semElementsSize (A := term)) H2.
         rewrite /seq_In -Hvars in H2.
         specialize (vars_with_type_Id _ _ _ H2); move => [x' ?]; subst.
         specialize (vars_with_type_le_length _ _ _ H2); move => H; subst.
@@ -232,26 +232,26 @@ Proof.
         inversion H2.
   - destruct (vars_with_type e (Arrow tau1 tau2)) as [| x e'] eqn:Hvars.
     + rewrite semLiftGenSize. intros t'. split.
-      * move => [t'' [/IHtau2 [H1 [H2 H3]] <-]]. 
+      * move => [t'' [/IHtau2 [H1 [H2 H3]] <-]].
         repeat split; auto; constructor; auto.
-      * move => [H1 [H2 H3]]. 
-        destruct t'; try now inversion H2. 
+      * move => [H1 [H2 H3]].
+        destruct t'; try now inversion H2.
         apply type_var in H1. rewrite Hvars in H1. inversion H1.
         eexists. split; last by reflexivity.
         apply IHtau2. inversion H1; subst. inversion H2; subst.
         repeat split; auto. inversion H3; auto.
     + rewrite semOneofSize. intros t. split.
       * move => [gen [[H1 | [H2 | //]] H]]; subst.
-        move /semLiftGenSize: H => [t' [/IHtau2 [H1 [H2 H3]] <-]]. 
-        repeat split; constructor; auto. 
+        move /semLiftGenSize: H => [t' [/IHtau2 [H1 [H2 H3]] <-]].
+        repeat split; constructor; auto.
         move /semElementsSize : H => H; subst. rewrite /seq_In -Hvars in H.
         destruct (vars_with_type_Id _ _ _ H) as [x' Heq]; subst.
         apply type_var in H. repeat split; auto; constructor.
       * intros [H1 [H2 H3]]. inversion H1; subst.
         eexists. split. right. left. reflexivity.
         apply semElementsSize. rewrite /seq_In -Hvars. apply type_var; auto.
-        eexists. split. left; reflexivity. 
-        apply semLiftGenSize. eexists. split; last by reflexivity. 
+        eexists. split. left; reflexivity.
+        apply semLiftGenSize. eexists. split; last by reflexivity.
         apply IHtau2; repeat split; auto. inversion H2; auto.
         inversion H3; auto.
         inversion H2.
@@ -261,12 +261,12 @@ Qed.
 Lemma gen_term_size_correct :
   forall (tau : type) (e : env) (n : nat) (s : nat),
     semGenSize (gen_term_size (n, tau) e) s <-->
-    [set t | 
+    [set t |
      (exists maxtau, typing_max_tau e t tau maxtau /\ maxtau <= s) /\
      Const_leq s t /\
      (exists h, app_no t = h /\ h <= n)].
 Proof.
-  move => tau e n s t. 
+  move => tau e n s t.
   replace tau with (snd (n, tau)); try reflexivity.
   have Heq :
     (exists h : nat, app_no t = h /\ h <= n) <->
@@ -274,10 +274,10 @@ Proof.
       simpl; split; auto.
   rewrite Heq.
   replace n with (fst (n, tau)) at 1; try reflexivity.
-  generalize (n, tau) e s t. clear Heq n tau e s t. 
-  change 
-    (forall (p : nat * type), 
-       (fun p => 
+  generalize (n, tau) e s t. clear Heq n tau e s t.
+  change
+    (forall (p : nat * type),
+       (fun p =>
           forall (e : env) (s : nat) (t : term),
             semGenSize (gen_term_size (fst p, snd p) e) s t <->
             (exists maxtau : nat, typing_max_tau e t (snd p) maxtau /\ maxtau <= s) /\
@@ -291,105 +291,111 @@ Proof.
       exists 0; split; try lia. apply app_free_app_no_0; auto.
     - destruct (vars_with_type e tau) eqn:Hvars;
       move /semOneofSize => [gen [[H1 | [H1 | //]] H2]]; subst;
-      try (move : H2=>  /semBindSize [tau' [ H2 /semBindSize 
-                                           [m [/semChooseSize H3 
-                                                /semBindSize 
-                                                [m' [/semChooseSize H4 
+      try (move : H2=>  /semBindSize [tau' [ H2 /semBindSize
+                                           [m [/semChooseSize H3
+                                                /semBindSize
+                                                [m' [/semChooseSize H4
                                                       /semLiftGen2Size H5]]]]]];
         move : H5 H2=> [[t1 t2] [[H5 H6] H7]]
                          /gen_type_correctSize H2;
         rewrite /set1 in H7; subst;
-        (apply (IH (n - m, Arrow tau' tau)) in H5; last by left; lia);
-        (apply (IH (n - m', tau')) in H6; last by left; lia);
-        move : H5 H6 => /= [[max1 [H5 Hle1]] [H6 [h1 [H7 H7']]]] 
+        (rewrite (IH (n - m, Arrow tau' tau)) in H5; last by left; lia);
+        (rewrite (IH (n - m', tau')) in H6; last by left; lia);
+        move : H5 H6 => /= [[max1 [H5 Hle1]] [H6 [h1 [H7 H7']]]]
                            [[max2 [H8 Hle2]] [H9 [h2 [H10 H10']]]]; subst;
         repeat (split; simpl; try now econstructor; eauto);
         [ exists (max (type_size tau') (max max1 max2));
             (split; try econstructor; eauto);
-            repeat (apply Max.max_lub; auto) | 
+            repeat (apply Max.max_lub; auto) |
           eexists; (split; first by reflexivity);
           unfold leq, super, OrdNat in H3, H4;
-          (have /andP [_ /leP Hle] : 0 <= m <= n by auto); 
+          (have /andP [_ /leP Hle] : 0 <= m <= n by auto);
           (have /andP [/leP Hle3 /leP Hle4]  : (n - m)%coq_nat <= m' <= n
             by apply H4; apply/leP; lia); lia ]);
-        try ( destruct tau; 
-              solve 
+        try ( destruct tau;
+              solve
                 [ move /semLiftGenSize : H2 => [t' [/arbNat_correctSize H2 H3]];
                     rewrite /set1 in H3; subst;
-                    repeat split; try constructor; auto; exists 0; 
+                    repeat split; try constructor; auto; exists 0;
                     split; auto; try lia; constructor
-                | move /semLiftGenSize : H2 => [t' [ H2 H3]]; 
-              rewrite /set1 in H3; subst; 
-              (apply (IH (n.+1, tau2)) in H2; last by 
+                | move /semLiftGenSize : H2 => [t' [ H2 H3]];
+              rewrite /set1 in H3; subst;
+              (rewrite (IH (n.+1, tau2)) in H2; last by
                    right; unfold lt_type; simpl; lia);
               move : H2 => /= [[maxt [H1 Hle]] [H2 [h [H3 H4]]]];
                     (repeat split; try now econstructor); eauto;
                     exists maxt; split; auto; constructor; auto ]).
-      move : H2 => [H2 | //]; subst.    
+      move : H2 => [H2 | //]; subst.
       move =>  /semElementsSize H. rewrite /seq_In -Hvars in H.
       specialize (vars_with_type_Id _ _ _ H); move => [x' ?]; subst.
       specialize (vars_with_type_le_length _ _ _ H); move => H1; subst.
-      apply type_var in H. repeat split; auto. 
+      apply type_var in H. repeat split; auto.
       exists 0; split. constructor. inversion H; auto. lia.
       constructor. exists 0. split; try lia. constructor. }
   { move => /= [[maxt [H1 Hle1]] [H2 [h [H3 Hle2]]]].
     destruct n.
     - apply gen_term_no_app_correctSize. destruct h; try lia.
-      repeat (split; auto); 
-        solve [apply typing_max_tau_correct; eexists; eauto | 
+      repeat (split; auto);
+        solve [apply typing_max_tau_correct; eexists; eauto |
                apply app_free_app_no_0; auto].
-    - destruct (vars_with_type e tau) eqn:Hvars; inversion H1; subst;
-      solve 
-        [ (have /type_var contra : (typing e(Id x) tau)
-            by apply typing_max_tau_correct; eexists; eauto);
-          rewrite Hvars in contra; now inversion contra
-        | apply semOneofSize; eexists; 
-          (split; first by right; left; reflexivity); apply semLiftGenSize;
-          eexists; (split; last by reflexivity); inversion H2; subst; 
-          apply arbNat_correctSize; lia
-        | apply semOneofSize; eexists; 
-          (split; first by right; left; reflexivity); apply semLiftGenSize;
-          eexists; (split; last by reflexivity); 
-          (apply (IH (n.+1, tau2)); first by right; unfold lt_type; simpl; lia);
-          inversion H2; inversion H1; subst; (repeat split; auto); simpl;
-          solve [eexists; split; eauto; simpl; eauto | 
-                 eexists; (split; first by reflexivity); simpl; auto ]
-        | apply semOneofSize; eexists; (split; first by left; reflexivity);
-          apply semBindSize; exists tau1; 
-          (split; first by apply gen_type_correctSize; eapply Max.max_lub_l; eauto);
-          simpl in Hle2; 
-          apply semBindSize; 
-          exists (n - (app_no t1)); 
-          (split; first by
-              apply semChooseSize; auto;
-              unfold leq, super, randomR, OrdNat;
-              apply/andP; split; apply/leP; lia);
-          apply semBindSize;
-          exists (n - (app_no t2));
-          (split; first by apply semChooseSize; auto;
-           unfold leq, super, randomR, OrdNat;
-           try (apply/leP; lia);
-             apply/andP; split; apply/leP; lia);
-          apply semLiftGen2Size;
-          exists (t1, t2); (split; last by reflexivity);
-          split => /=;
-          [ apply (IH (n - (n - app_no t1)%coq_nat, Arrow tau1 tau)) |
-            apply (IH (n - (n - app_no t2)%coq_nat, tau1)) ];
-            try (left; lia);
-            inversion H2; subst; repeat (split; auto);
-            solve [ inversion H; subst; eexists; split; eauto; try lia;
-                    (try now eapply Max.max_lub_l; eapply Max.max_lub_r; eauto);
-                    try (now eapply Max.max_lub_r; eapply Max.max_lub_r; eauto) |
-                   eexists; split; eauto; simpl in Hle2; simpl; lia ]
-        | apply semOneofSize; eexists; 
-          (split; first by right; right; left; reflexivity);
-          apply semElementsSize; rewrite /seq_In -Hvars;
-          apply type_var; apply typing_max_tau_correct; eexists; eauto ]. }
-Qed. 
+    - destruct (vars_with_type e tau) eqn:Hvars; inversion H1; subst.
+      { have /type_var contra : (typing e(Id x) tau) by apply typing_max_tau_correct; eexists; eauto.
+        rewrite Hvars in contra; now inversion contra. }
+      all: setrw @semOneofSize.
+      1,5: eexists; split; [ right; left; reflexivity | ];
+        setrw @semLiftGenSize;
+        eexists; (split; last by reflexivity); inversion H2; subst;
+        apply arbNat_correctSize; lia.
+      { eexists; split; first by right; left; reflexivity.
+        setrw @semLiftGenSize.
+        eexists; (split; last by reflexivity).
+        rewrite (IH (n.+1, tau2)); cbn; [ | right; unfold lt_type; simpl; lia ].
+        inversion H2; inversion H1; subst; (repeat split; auto); simpl;
+        solve [eexists; split; eauto; simpl; eauto |
+               eexists; (split; first by reflexivity); simpl; auto ]. }
+      1,4: eexists; split; [ left; reflexivity | ];
+        setrw semBindSize; exists tau1;
+        split; [ apply gen_type_correctSize; eapply Max.max_lub_l; eauto | ];
+        simpl in Hle2;
+        setrw semBindSize;
+        exists (n - (app_no t1));
+        split; [
+            apply semChooseSize; auto;
+            unfold leq, super, randomR, OrdNat;
+            apply/andP; split; apply/leP; lia | ];
+        setrw semBindSize;
+        exists (n - (app_no t2));
+        split; [ apply semChooseSize; auto;
+         unfold leq, super, randomR, OrdNat;
+         try (apply/leP; lia);
+           apply/andP; split; apply/leP; lia | ];
+        setrw @semLiftGen2Size;
+        exists (t1, t2); (split; [ | reflexivity ]);
+        split => /=;
+        [ rewrite (IH (n - (n - app_no t1)%coq_nat, Arrow tau1 tau)) |
+          rewrite (IH (n - (n - app_no t2)%coq_nat, tau1)) ];
+          try (left; lia);
+          inversion H2; subst; repeat (split; auto);
+          solve [ inversion H; subst; eexists; split; eauto; try lia;
+                  (try now eapply Max.max_lub_l; eapply Max.max_lub_r; eauto);
+                  try (now eapply Max.max_lub_r; eapply Max.max_lub_r; eauto) |
+                 eexists; split; eauto; simpl in Hle2; simpl; lia ].
+      { eexists; (split; first by right; right; left; reflexivity);
+        setrw @semElementsSize; rewrite /seq_In -Hvars;
+        apply type_var; apply typing_max_tau_correct; eexists; eauto. }
+      { eexists; split; first by right; left; reflexivity.
+        setrw @semLiftGenSize.
+        eexists; (split; last by reflexivity).
+        rewrite (IH (n.+1, tau2)); cbn; [ | right; unfold lt_type; simpl; lia ].
+        inversion H2; inversion H1; subst; (repeat split; auto); simpl;
+        solve [eexists; split; eauto; simpl; eauto |
+               eexists; (split; first by reflexivity); simpl; auto ]. }
+  }
+Qed.
 
 Lemma gen_term_correct :
   forall (tau : type),
-    semGen (gen_term tau) <--> [set t | typing nil t tau]. 
+    semGen (gen_term tau) <--> [set t | typing nil t tau].
 Proof.
   intros.
   unfold gen_term. rewrite semSized => t. split.
@@ -397,10 +403,10 @@ Proof.
     apply typing_max_tau_correct. eexists; eauto.
   - move => /typing_max_tau_correct [m Ht].
     eexists (max m (max (app_no t) (max_const t))). split.
-    reflexivity. apply gen_term_size_correct. 
-    repeat split. exists m. split; auto. apply Max.le_max_l. 
+    reflexivity. apply gen_term_size_correct.
+    repeat split. exists m. split; auto. apply Max.le_max_l.
     eapply Const_leq_trans; last by apply max_const_Const_leq.
     eapply PeanoNat.Nat.max_le_iff. right. apply Max.le_max_r.
-    eexists; split. reflexivity. 
+    eexists; split. reflexivity.
     eapply PeanoNat.Nat.max_le_iff. right. apply Max.le_max_l.
 Qed.
