src/RandomSplitMix.v
@@ -1,0 +1,11 @@
+From QuickChick Require Import SplitMix.
+From QuickChick Require Export Random.
+
+Definition seed := SplitMix.state.
+
+CoFixpoint generate (s : seed) : random :=
+  {| split := fun _ => let '(s1, s2) := SplitMix.split s in (generate s1, generate s2)
+  ;  bits := fun _ => SplitMix.bits s
+  |}.
+Definition split_seed : seed -> seed * seed := SplitMix.split.
+Parameter new_seed : unit -> seed.
