test/internal/test_extraction.v
@@ -1,0 +1,99 @@
+From Coq Require Import ZArith NArith String Int63 Extraction ExtrOcamlZBigInt.
+From QuickChick Require Import QuickChick.
+
+From SimpleIO Require Import SimpleIO.
+Import IO.Notations.
+
+RunIOPackage "zarith".
+
+Definition assert_equal {A} `{Dec_Eq A} `{Show A} (x y : A) : IO unit :=
+  if dec_eq x y then ret tt else print_endline ("Failed: " ++ show (x, y))%string.
+
+Definition test_div_ : unit :=
+  let _ : (1 / (-3) = -1)%Z := eq_refl in
+  let _ : ((-1) / (-3) = 0)%Z := eq_refl in
+  let _ : ((-1) / 3 = (-1))%Z := eq_refl in
+  tt.
+
+Definition test_div : IO unit :=
+  ( assert_equal (1 / (-3)) (-1) ;;
+    assert_equal ((-1) / (-3)) 0 ;;
+    assert_equal ((-1) / 3) (-1)
+  )%Z%io.
+
+Definition test_mod_ : unit :=
+  let _ : (1 mod (-3) = -2)%Z := eq_refl in
+  let _ : ((-1) mod (-3) = -1)%Z := eq_refl in
+  let _ : ((-1) mod 3 = 2)%Z := eq_refl in
+  tt.
+
+Definition test_mod : IO unit :=
+  ( assert_equal (1 mod (-3)) (-2) ;;
+    assert_equal ((-1) mod (-3)) (-1) ;;
+    assert_equal ((-1) mod 3) 2
+  )%Z%io.
+
+Definition test_shiftr_ : unit :=
+  let _ : (Z.shiftr 3 1 = 1)%Z := eq_refl in
+  let _ : (Z.shiftr 3 (-1) = 6)%Z := eq_refl in
+  let _ : (Z.shiftr (-3) 1 = -2)%Z := eq_refl in
+  let _ : (Z.shiftr (-3) (-1) = -6)%Z := eq_refl in
+  tt.
+
+Definition test_shiftr : IO unit :=
+  ( assert_equal (Z.shiftr 3 1) 1 ;;
+    assert_equal (Z.shiftr 3 (-1)) 6 ;;
+    assert_equal (Z.shiftr (-3) 1) (-2) ;;
+    assert_equal (Z.shiftr (-3) (-1)) (-6)
+  )%Z%io.
+
+Definition test_shiftl_ : unit :=
+  let _ : (Z.shiftl 3 1 = 6)%Z := eq_refl in
+  let _ : (Z.shiftl 3 (-1) = 1)%Z := eq_refl in
+  let _ : (Z.shiftl (-3) 1 = -6)%Z := eq_refl in
+  let _ : (Z.shiftl (-3) (-1) = -2)%Z := eq_refl in
+  tt.
+
+Definition test_shiftl : IO unit :=
+  ( assert_equal (Z.shiftl 3 1) 6 ;;
+    assert_equal (Z.shiftl 3 (-1)) 1 ;;
+    assert_equal (Z.shiftl (-3) 1) (-6) ;;
+    assert_equal (Z.shiftl (-3) (-1)) (-2)
+  )%Z%io.
+
+Definition is_left {A B} (x : {A} + {B}) : bool :=
+  match x with
+  | left _ => true
+  | right _ => false
+  end.
+
+Definition test_misc_Z : IO unit :=
+  ( assert_equal (Z.eqb 0%Z 1%Z) false ;;
+    assert_equal (is_left (Z.eq_dec 0%Z 1%Z)) false ;;
+    assert_equal (Z.div_eucl 17 5) (3, 2)%Z ;;
+    assert_equal (Z.div_eucl (-17) (-5)) (3, -2)%Z ;;
+    assert_equal (Z.to_N 3%Z) 3%N ;;
+    assert_equal (Z.to_N (-1)%Z) 0%N ;;
+    assert_equal (Int63.to_Z (Int63.of_Z 0)) 0%Z
+  )%io.
+
+Definition test_misc_N : IO unit :=
+  ( assert_equal (N.eqb 0%N 1%N) false ;;
+    assert_equal (is_left (N.eq_dec 0%N 1%N)) false ;;
+    assert_equal (N.div_eucl 17 5) (3, 2)%N ;;
+    assert_equal (N.div 10 2) 5%N ;;
+    assert_equal (N.modulo 17 5) 2%N ;;
+    assert_equal (N.shiftl 10 1) 20%N ;;
+    assert_equal (N.shiftr 10 1) 5%N
+  )%io.
+
+Definition test_all : IO unit :=
+  ( test_div ;;
+    test_mod ;;
+    test_shiftr ;;
+    test_shiftl ;;
+    test_misc_Z ;;
+    test_misc_N
+  )%io.
+
+RunIO test_all.
