test/internal/test_splitmix.v
@@ -1,0 +1,45 @@
+(** Test SplitMix implementation against some hardcoded result *)
+
+From Coq Require Import List ZArith.
+From QuickChick Require Import SplitMix QuickChick.
+
+Import CoqInt64.
+Import ListNotations.
+
+Definition next (s : state) : int64 * state :=
+  let g := gamma s in
+  let s1 := (seed s + g)%int64 in
+  (mix64_variant13 s1, SplitMix.MkState s1 g).
+
+Definition example : list int64 :=
+  let split := SplitMix.split in
+  let g0 := of_seed 33 in
+  let '(n0, g0) := next g0 in
+  let '(n1, g0) := next g0 in
+  let '(g1, _g0) := split g0 in
+  let '(n2, g1) := next g1 in
+  let '(g2, g1) := split g1 in
+  let '(n3, g1) := next g1 in
+  let '(g3, g2) := split g2 in
+  let '(n4, g2) := next g2 in
+  let '(n5, g2) := next g2 in
+  let '(n6, g3) := next g3 in
+  let '(n7, g3) := next g3 in
+  let '(n8, g3) := next g3 in
+  (* Run mix_gamma many times to trigger the gamma-fixing branch. *)
+  let g3' := Z.iter 300 (fun g => let '(g, _) := split g in g) g3 in
+  let '(n9, _g3) := next g3' in
+  [n0; n1; n2; n3; n4; n5; n6; n7; n8; n9].
+
+Lemma example_correct : example =
+  [ 3174492301114349736
+  ; 1387786489429541378
+  ; 2612135949649290519
+  ; -6594435460564017959
+  ; 6114845654480584590
+  ; -3434961282303982149
+  ; -4710980162942128616
+  ; -5883331640739962744
+  ; 7437753320184232638
+  ; -2875907909505887564 ]%int64.
+Proof. cbv. reflexivity. Qed.
