test/mutation/run.sh
@@ -3,8 +3,10 @@ set -e
 MUTATION=mutation
 
 # Extract and compile the example
-coqc -Q ../../src QuickChick ${MUTATION}.v
-ocamlbuild -pkg zarith ${MUTATION}.native
+coqc ${MUTATION}.v
+EXTRACTED=mutation.ml
+sed 's/Uint63.of_int//g' -i ${EXTRACTED}
+ocamlbuild -pkg zarith -pkg pure-splitmix ${MUTATION}.native
 
 # Look for mutants and test them
 PATH=../../scripts:$PATH quickchick ./${MUTATION}.native 4
