test/plugin/run.sh
@@ -2,4 +2,4 @@
 set -e
 
 # Just test this compiles
-coqc -Q ../../src QuickChick plugin.v
+coqc plugin.v
